feat(DybjerOrd): implement basic relation properties and Setoid for DPreOrd

OrdinalsInductionRecursion/DybjerOrd/PreOrd.lean
@@ -34,4 +34,135 @@ inductive DMem : DPreOrd → DPreOrd → Prop where
       DMem x (f a) → DMem x (.sup c f)
 end
 
+instance : Membership DPreOrd DPreOrd := ⟨DMem⟩
+instance : HasSubset DPreOrd := ⟨DSubset⟩
+
+/-- Igualdad extensional (equivalencia) de pre-ordinales -/
+def Equiv (x y : DPreOrd) : Prop := DSubset x y ∧ DSubset y x
+
+-- ==========================================
+-- Lemas de Equivalencia (Setoid)
+-- ==========================================
+
+theorem DSubset_sup {y z : DPreOrd} {A : Type} {c : UCodeFam A} {f : A → DPreOrd}
+  (h : DSubset y z) (a : A) (hz : z = f a) :
+    DSubset y (.sup c f)
+      :=
+  match y, z, h with
+  | _, _, .zero_subset _ => .zero_subset _
+  | _, _, .succ_subset hmem => .succ_subset (DMem.mem_sup a (hz ▸ hmem))
+  | _, _, .sup_subset hsub => .sup_subset fun k => DSubset_sup (hsub k) a hz
+
+theorem DSubset_refl
+  (x : DPreOrd) :
+    DSubset x x
+      :=
+  match x with
+  | .zero => .zero_subset _
+  | .succ x' => .succ_subset (.mem_succ (DSubset_refl x'))
+  | .sup _c f => .sup_subset fun a => DSubset_sup (DSubset_refl (f a)) a rfl
+
+theorem DMem_self_succ
+  (x : DPreOrd) :
+    DMem x (.succ x)
+      :=
+  .mem_succ (DSubset_refl x)
+
+def trans_all
+  (x : DPreOrd) :
+    (∀ {y z}, DSubset x y → DSubset y z → DSubset x z) ∧
+    (∀ {y z}, DMem x y → DSubset y z → DMem x z) ∧
+    (∀ {y z}, DSubset x y → DMem y z → DMem x z)
+      :=
+  let sub_sub : ∀ {y z}, DSubset x y → DSubset y z → DSubset x z :=
+    match x with
+    | .zero => fun _ _ => .zero_subset _
+    | .succ x' => fun h1 h2 =>
+      match h1 with
+      | @DSubset.succ_subset _ _ hmem1 => .succ_subset ((trans_all x').2.1 hmem1 h2)
+    | .sup _c f => fun h1 h2 =>
+      match h1 with
+      | @DSubset.sup_subset _ _ _ _ hsub1 => .sup_subset fun a => (trans_all (f a)).1 (hsub1 a) h2
+
+  let rec sub_mem {y z} (h1 : DSubset x y) (h2 : DMem y z) : DMem x z :=
+    match y, z, h2 with
+    | _, _, .mem_succ hsub2 => .mem_succ (sub_sub h1 hsub2)
+    | _, _, .mem_sup a hmem2 => .mem_sup a (sub_mem h1 hmem2)
+
+  let rec mem_sub {y z} (h1 : DMem x y) (h2 : DSubset y z) : DMem x z :=
+    match y, z, h2 with
+    | _, _, .zero_subset _ => nomatch h1
+    | _, _, @DSubset.succ_subset y' _ hmem2 =>
+      match h1 with
+      | @DMem.mem_succ _ _ hsub1 => sub_mem hsub1 hmem2
+    | _, _, @DSubset.sup_subset _ _ _ _ hsub2 =>
+      match h1 with
+      | @DMem.mem_sup _ _ _ _ a hmem1 => mem_sub hmem1 (hsub2 a)
+
+  ⟨sub_sub, mem_sub, sub_mem⟩
+
+theorem DSubset_trans {x y z : DPreOrd} (h1 : DSubset x y) (h2 : DSubset y z) : DSubset x z :=
+  (trans_all x).1 h1 h2
+
+theorem DMem_DSubset_trans {x y z : DPreOrd} (h1 : DMem x y) (h2 : DSubset y z) : DMem x z :=
+  (trans_all x).2.1 h1 h2
+
+theorem DSubset_DMem_trans {x y z : DPreOrd} (h1 : DSubset x y) (h2 : DMem y z) : DMem x z :=
+  (trans_all x).2.2 h1 h2
+
+def trans_y (y : DPreOrd) :
+  (DSubset y (.succ y)) ∧
+  (∀ {x}, DMem x y → DSubset x y) :=
+  match y with
+  | .zero =>
+    ⟨DSubset.zero_subset _, fun h => nomatch h⟩
+  | .succ a =>
+    let ih := trans_y a
+    let self_succ := DSubset.succ_subset (DMem.mem_succ ih.1)
+    let rec sub_succ_a {x} (h : DSubset x a) : DSubset x (.succ a) :=
+      match x, h with
+      | _, DSubset.zero_subset _ => DSubset.zero_subset _
+      | _, @DSubset.succ_subset z _ hmem =>
+        DSubset.succ_subset (DMem.mem_succ (ih.2 hmem))
+      | _, @DSubset.sup_subset _ _ _ _ hsub =>
+        DSubset.sup_subset fun j => sub_succ_a (hsub j)
+    let mem_sub := fun {x} (h : DMem x (.succ a)) =>
+      match x, h with
+      | _, DMem.mem_succ hsub => sub_succ_a hsub
+    ⟨self_succ, mem_sub⟩
+  | .sup c f =>
+    let ih := fun i => trans_y (f i)
+    let mem_sub := fun {x} (h : DMem x (.sup c f)) =>
+      match x, h with
+      | _, DMem.mem_sup i hmem => DSubset_sup ((ih i).2 hmem) i rfl
+    let rec sub_succ_sup {x} (h : DSubset x (.sup c f)) : DSubset x (.succ (.sup c f)) :=
+      match x, h with
+      | _, DSubset.zero_subset _ => DSubset.zero_subset _
+      | _, @DSubset.succ_subset z _ hmem =>
+        DSubset.succ_subset (DMem.mem_succ (mem_sub hmem))
+      | _, @DSubset.sup_subset _ _ _ _ hsub =>
+        DSubset.sup_subset fun j => sub_succ_sup (hsub j)
+    let self_succ := DSubset.sup_subset fun i => sub_succ_sup (DSubset_sup (DSubset_refl _) i rfl)
+    ⟨self_succ, mem_sub⟩
+
+theorem Dmem_implies_subset {x y : DPreOrd} (h : DMem x y) : DSubset x y :=
+  (trans_y y).2 h
+
+theorem Equiv_refl (x : DPreOrd) : Equiv x x :=
+  ⟨DSubset_refl x, DSubset_refl x⟩
+
+theorem Equiv_symm {x y : DPreOrd} (h : Equiv x y) : Equiv y x :=
+  ⟨h.right, h.left⟩
+
+theorem Equiv_trans {x y z : DPreOrd} (h1 : Equiv x y) (h2 : Equiv y z) : Equiv x z :=
+  ⟨DSubset_trans h1.left h2.left, DSubset_trans h2.right h1.right⟩
+
+instance Setoid : Setoid DPreOrd where
+  r := Equiv
+  iseqv := {
+    refl := Equiv_refl
+    symm := Equiv_symm
+    trans := Equiv_trans
+  }
+
 end DybjerOrd
